Debug.lean
@@ -1,6 +1,0 @@
-import Sodium.FFI
-
-open Lean Sodium FFI
-
-def main : IO Unit := do
-  return
